do_commute method to swap two adjacent transitions

examples/concurrency-strategies/commutativity-strategy.dfy
@@ -74,20 +74,46 @@ module Concrete {
       // we're done! exit the runnable queue
       && s'.threads == MapRemove1(s.threads, tid)
       && ui == Some(Abstract.DonateOp(t.victim, None))
-    else if LockFree(s, nextLock) then
-      var t' := Thread(nextLock, t.victim);
+    else
+      && LockFree(s, nextLock)
+      && var t' := Thread(nextLock, t.victim);
       && s'.board == s.board
       && s'.threads == s.threads[tid := t']
-      && ui == None
-    else
-      // Need to advance, but waiting on a lock
-      && s' == s
       && ui == None
   }
 
   predicate Next(s:State, s':State, tid: int, ui:Abstract.UI) {
     || (exists victim :: Start(s, s', victim, tid, ui))
     || Advance(s, s', tid, ui)
+  }
+
+  predicate LocksDistinct(s: State, tid1: int, tid2: int)
+  {
+    tid1 in s.threads && tid2 in s.threads && tid1 != tid2 ==>
+        s.threads[tid1].lockHeld != s.threads[tid2].lockHeld
+  }
+
+  predicate Inv(s: State)
+  {
+    && (forall tid1, tid2 :: LocksDistinct(s, tid1, tid2))
+  }
+
+  lemma InitImpliesInv(s: State)
+  requires Init(s)
+  ensures Inv(s)
+  {
+  }
+
+  lemma NextPreservesInv(s: State, s': State, tid: int, ui: Abstract.UI)
+  requires Inv(s)
+  requires Next(s, s', tid, ui)
+  ensures Inv(s')
+  {
+    forall tid1, tid2
+    ensures LocksDistinct(s', tid1, tid2)
+    {
+      assert LocksDistinct(s, tid1, tid2);
+    }
   }
 }
 
@@ -96,154 +122,415 @@ module ConcreteOrdered {
   import Abstract
   import opened Options
 
-  datatype Variables = Variables(
-      state: Concrete.State,
-      orders: map<int, int>
-  )
+  datatype Lock = HasLock(lock: int)
+                | NotStarted
+                | Done
 
-  predicate Next(s: Variables, s': Variables, tid: int, ui:Abstract.UI, my_rank: int)
+  datatype LockTrans = LockTrans(from: Lock, to: Lock)
+
+  predicate lt_less(a: LockTrans, b: LockTrans)
   {
-    && Concrete.Next(s.state, s'.state, tid, ui)
-    && (tid !in s.state.threads && tid in s'.state.threads ==>
-      s'.orders == s.orders[tid := my_rank]
+    && (a.from.HasLock? && b.from.HasLock? ==> a.from.lock < b.from.lock)
+    && (a.from.HasLock? && b.to.HasLock? ==> a.from.lock < b.to.lock)
+    && (a.to.HasLock? && b.from.HasLock? ==> a.to.lock < b.from.lock)
+    && (a.to.HasLock? && b.to.HasLock? ==> a.to.lock < b.to.lock)
+  }
+
+  predicate Next(s: Concrete.State, s': Concrete.State, tid: int,
+      ui:Abstract.UI, lt: LockTrans)
+  {
+    && Concrete.Next(s, s', tid, ui)
+    && (lt.from ==
+      if tid in s.threads
+        then HasLock(s.threads[tid].lockHeld)
+        else NotStarted
     )
-    && (tid in s.state.threads && tid !in s'.state.threads ==>
-      && s'.orders == Concrete.MapRemove1(s.orders, tid)
-    )
-    && (tid !in s.state.threads && tid !in s'.state.threads ==>
-      && s'.orders == s.orders
-    )
-    && (tid in s.state.threads && tid in s'.state.threads ==>
-      && tid in s.orders
-      && s.orders[tid] == my_rank
-      && s'.orders == s.orders
+    && (lt.to ==
+      if tid in s'.threads
+        then HasLock(s'.threads[tid].lockHeld)
+        else Done
     )
   }
 
-  predicate ThreadsOrdered(s: Variables, tid1: int, tid2: int)
-  {
-    tid1 in s.orders && tid2 in s.orders && s.orders[tid1] < s.orders[tid2] ==>
-      && tid1 in s.state.threads
-      && tid2 in s.state.threads
-      && s.state.threads[tid1].lockHeld < s.state.threads[tid2].lockHeld
-  }
-
-  predicate LocksDistinct(s: Variables, tid1: int, tid2: int)
-  {
-    tid1 in s.state.threads && tid2 in s.state.threads && tid1 != tid2 ==>
-        s.state.threads[tid1].lockHeld != s.state.threads[tid2].lockHeld
-  }
-
-  predicate Inv(s: Variables)
-  {
-    && (forall tid1, tid2 :: ThreadsOrdered(s, tid1, tid2))
-    && (forall tid1, tid2 :: LocksDistinct(s, tid1, tid2))
-  }
-
-  lemma Commute(s: Variables, s1: Variables, s12: Variables,
-      tid1: int, ui1: Abstract.UI, my_rank1: int,
-      tid2: int, ui2: Abstract.UI, my_rank2: int)
-  returns (s2: Variables)
-  requires Inv(s)
-  requires Inv(s1)
-  requires Inv(s12)
-  requires Next(s, s1, tid1, ui1, my_rank1)
-  requires Next(s1, s12, tid2, ui2, my_rank2)
-  requires my_rank1 > my_rank2
+  lemma Commute(s: Concrete.State, s1: Concrete.State, s12: Concrete.State,
+      tid1: int, ui1: Abstract.UI, lt1: LockTrans,
+      tid2: int, ui2: Abstract.UI, lt2: LockTrans)
+  returns (s2: Concrete.State)
+  requires Concrete.Inv(s)
+  requires Concrete.Inv(s1)
+  requires Concrete.Inv(s12)
+  requires Next(s, s1, tid1, ui1, lt1)
+  requires Next(s1, s12, tid2, ui2, lt2)
+  requires lt_less(lt1, lt2)
   requires tid1 != tid2
-  requires !(
-      && tid1 in s1.state.threads && s1.state.threads[tid1].lockHeld == 0
-      && tid2 in s12.state.threads && s12.state.threads[tid2].lockHeld == 0
-    )
-  ensures Next(s, s2, tid2, ui2, my_rank2)
-  ensures Next(s2, s12, tid1, ui1, my_rank1)
+  ensures Next(s, s2, tid2, ui2, lt2)
+  ensures Next(s2, s12, tid1, ui1, lt1)
   {
-    assert ThreadsOrdered(s, tid2, tid1);
-    assert LocksDistinct(s, tid1, tid2);
+    assert Concrete.LocksDistinct(s, tid1, tid2);
 
-    if Concrete.Advance(s1.state, s12.state, tid2, ui2) {
-      var t := s.state.threads[tid2];
-      assert t == s1.state.threads[tid2];
-      assert s.state.board[t.lockHeld] == s1.state.board[t.lockHeld];
+    if Concrete.Advance(s1, s12, tid2, ui2) {
+      var t := s.threads[tid2];
+      assert t == s1.threads[tid2];
+      assert s.board[t.lockHeld] == s1.board[t.lockHeld];
 
       var nextLock := t.lockHeld + 1;
-      if s.state.board[t.lockHeld].stones == t.victim {
+      if s.board[t.lockHeld].stones == t.victim {
         // yay we found it!
-        var board := s.state.board[t.lockHeld := s.state.board[t.lockHeld].(stones := t.victim + 1)];
-        var threads := Concrete.MapRemove1(s.state.threads, tid2);
-        var orders := Concrete.MapRemove1(s.orders, tid2);
-        s2 := Variables(Concrete.State(board, threads), orders);
+        var board := s.board[t.lockHeld := s.board[t.lockHeld].(stones := t.victim + 1)];
+        var threads := Concrete.MapRemove1(s.threads, tid2);
+        s2 := Concrete.State(board, threads);
 
         assert ui2.Some?;
         assert ui2.value.victim == t.victim;
         assert ui2.value.outidx == Some(t.lockHeld);
-        assert Concrete.Advance(s.state, s2.state, tid2, ui2);
-        assert Next(s, s2, tid2, ui2, my_rank2);
-      } else if |s.state.board| <= nextLock {
-        var board := s.state.board;
-        var threads := Concrete.MapRemove1(s.state.threads, tid2);
-        var orders := Concrete.MapRemove1(s.orders, tid2);
-        s2 := Variables(Concrete.State(board, threads), orders);
+        assert Concrete.Advance(s, s2, tid2, ui2);
+        assert Next(s, s2, tid2, ui2, lt2);
+      } else if |s.board| <= nextLock {
+        var board := s.board;
+        var threads := Concrete.MapRemove1(s.threads, tid2);
+        s2 := Concrete.State(board, threads);
 
-        assert Next(s, s2, tid2, ui2, my_rank2);
-      } else if Concrete.LockFree(s.state, nextLock) {
-        var t' := Concrete.Thread(nextLock, t.victim);
-        var board := s.state.board;
-        var threads := s.state.threads[tid2 := t'];
-        var orders := s.orders;
-        s2 := Variables(Concrete.State(board, threads), orders);
-
-        assert Next(s, s2, tid2, ui2, my_rank2);
+        assert Next(s, s2, tid2, ui2, lt2);
       } else {
-        var board := s.state.board;
-        var threads := s.state.threads;
-        var orders := s.orders;
-        s2 := Variables(Concrete.State(board, threads), orders);
+        var t' := Concrete.Thread(nextLock, t.victim);
+        var board := s.board;
+        var threads := s.threads[tid2 := t'];
+        s2 := Concrete.State(board, threads);
 
-        assert Next(s, s2, tid2, ui2, my_rank2);
+        assert Concrete.LockFree(s1, nextLock);
+        assert lt2.to == HasLock(nextLock);
+        forall id | id in s.threads
+        ensures s.threads[id].lockHeld != nextLock
+        {
+          if id == tid1 {
+            assert s.threads[id].lockHeld != nextLock;
+          } else {
+            assert s.threads[id].lockHeld
+                == s1.threads[id].lockHeld;
+            assert s.threads[id].lockHeld != nextLock;
+          }
+        }
+        assert Concrete.LockFree(s, nextLock);
+
+        assert Concrete.Advance(s, s2, tid2, ui2);
+        assert Next(s, s2, tid2, ui2, lt2);
       }
     } else {
-      var victim :| Concrete.Start(s1.state, s12.state, victim, tid2, ui2);
-      var board := s.state.board;
+      var victim :| Concrete.Start(s1, s12, victim, tid2, ui2);
+      var board := s.board;
       var newThread := Concrete.Thread(0, victim);
-      var threads := s.state.threads[tid2 := newThread];
-      var orders := s.orders[tid2 := my_rank2];
-      s2 := Variables(Concrete.State(board, threads), orders);
+      var threads := s.threads[tid2 := newThread];
+      s2 := Concrete.State(board, threads);
 
-      forall id | id in s.state.threads
-      ensures s.state.threads[id].lockHeld != 0
+      forall id | id in s.threads
+      ensures s.threads[id].lockHeld != 0
       {
-        assert LocksDistinct(s, id, tid1);
-        assert LocksDistinct(s, id, tid2);
-        assert id != tid2;
         if id == tid1 {
-          if s.state.threads[tid1].lockHeld == 0 {
-            assert ThreadsOrdered(s12, tid2, tid1);
-            assert tid1 in s1.state.threads;
-            assert s1.state.threads[tid1].lockHeld == 0;
-            assert tid2 in s12.state.threads;
-            assert s12.state.threads[tid2].lockHeld == 0;
-            assert false;
-          }
-          // Ordering is used here:
-          //assert s12.state.threads[tid1].lockHeld
-          //    > s12.state.threads[tid2].lockHeld;
-          //assert s1.state.threads[tid1].lockHeld
-          //    == s.state.threads[tid1].lockHeld;
+          assert s.threads[id].lockHeld != 0;
         } else {
-          assert s1.state.threads[id].lockHeld
-              == s.state.threads[id].lockHeld;
+          assert s.threads[id].lockHeld
+              == s1.threads[id].lockHeld;
+          assert s.threads[id].lockHeld != 0;
         }
       }
-      assert Concrete.Start(s.state, s2.state, victim, tid2, ui2);
-      assert Next(s, s2, tid2, ui2, my_rank2);
+
+      assert Concrete.Start(s, s2, victim, tid2, ui2);
+      assert Next(s, s2, tid2, ui2, lt2);
     }
 
-    assert Next(s2, s12, tid1, ui1, my_rank1);
+    if Concrete.Advance(s, s1, tid1, ui1) {
+      assert Concrete.Advance(s2, s12, tid1, ui1);
+      assert Next(s2, s12, tid1, ui1, lt1);
+    } else {
+      var victim :| Concrete.Start(s, s1, victim, tid1, ui1);
+      assert Concrete.Start(s2, s12, victim, tid1, ui1);
+      assert Next(s2, s12, tid1, ui1, lt1);
+    }
   }
 }
 
 module TheoremProof {
+  import Abstract
+  import Concrete
+  import ConcreteOrdered
+
+  datatype Edge = Edge(
+      ui: Abstract.UI,
+      tid: int
+  )
+
+  datatype Trace = Behavior(
+      states: seq<Concrete.State>,
+      edges: seq<Edge>
+  )
+
+  datatype SEdge = SEdge(
+      ui: Abstract.UI,
+      lt: ConcreteOrdered.LockTrans,
+      tid: int,
+      order: int
+  )
+
+  datatype SState = SState(
+    state: Concrete.State,
+    thread_map: map<int, int>,
+    largest_so_far: int
+  )
+
+  datatype STrace = STrace(
+    states: seq<SState>,
+    edges: seq<SEdge>
+  )
+
+  predicate ThreadMapUpdate(s: SState, s': SState, tid: int, order: int)
+  {
+    if tid in s.state.threads then (
+      if tid in s'.state.threads then (
+        && s'.thread_map == s.thread_map
+        && s'.largest_so_far == s.largest_so_far
+        && tid in s.thread_map
+        && order == s.thread_map[tid]
+      ) else (
+        && s'.thread_map == Concrete.MapRemove1(s.thread_map, tid)
+        && s'.largest_so_far == s.largest_so_far
+        && tid in s.thread_map
+        && order == s.thread_map[tid]
+      )
+    ) else (
+      if tid in s'.state.threads then (
+        && s'.thread_map == s.thread_map[tid := s.largest_so_far + 1]
+        && s'.largest_so_far == s.largest_so_far + 1
+        && order == s.largest_so_far + 1
+      ) else (
+        && s'.thread_map == s.thread_map
+        && s'.largest_so_far == s.largest_so_far + 1
+        && order == s.largest_so_far + 1
+      )
+    )
+  }
+
+  predicate WFSTraceAt(trace: STrace, i: int)
+  requires 0 <= i < |trace.edges|
+  requires i+1 < |trace.states|
+  {
+    && ConcreteOrdered.Next(
+      trace.states[i].state,
+      trace.states[i+1].state, 
+      trace.edges[i].tid,
+      trace.edges[i].ui,
+      trace.edges[i].lt
+    )
+    && ThreadMapUpdate(
+      trace.states[i],
+      trace.states[i+1],
+      trace.edges[i].tid,
+      trace.edges[i].order
+    )
+  }
+
+  predicate WFSTrace(trace: STrace)
+  {
+    && |trace.states| == |trace.edges| + 1
+    && Concrete.Init(trace.states[0].state)
+    && (forall i | 0 <= i < |trace.edges| :: WFSTraceAt(trace, i))
+    && trace.states[0].thread_map == map[]
+  }
+
+  lemma inv_at(trace: STrace, i: int)
+  requires WFSTrace(trace)
+  requires 0 <= i < |trace.states|
+  ensures Concrete.Inv(trace.states[i].state)
+  {
+    if (i == 0) {
+      Concrete.InitImpliesInv(trace.states[0].state);
+    } else {
+      inv_at(trace, i-1);
+      assert WFSTraceAt(trace, i-1);
+      Concrete.NextPreservesInv(
+          trace.states[i-1].state,
+          trace.states[i].state,
+          trace.edges[i-1].tid,
+          trace.edges[i-1].ui);
+    }
+  }
+
+  lemma le_largest_so_far(trace: STrace, i: int, tid: int)
+  requires WFSTrace(trace)
+  requires 0 <= i < |trace.states|
+  requires tid in trace.states[i].thread_map
+  ensures trace.states[i].thread_map[tid] <= trace.states[i].largest_so_far
+  {
+    if i == 0 {
+    } else {
+      assert WFSTraceAt(trace, i-1);
+      if tid in trace.states[i-1].thread_map {
+        le_largest_so_far(trace, i-1, tid);
+      } else {
+      }
+    }
+  }
+
+  lemma order_le_largest_so_far(trace: STrace, i: int)
+  requires WFSTrace(trace)
+  requires 0 <= i < |trace.edges|
+  ensures trace.edges[i].order <= trace.states[i+1].largest_so_far
+  {
+    var tid := trace.edges[i].tid;
+    assert WFSTraceAt(trace, i);
+    if tid in trace.states[i].thread_map {
+      le_largest_so_far(trace, i, tid);
+    } else {
+    }
+  }
+
+  lemma lock_order(trace: STrace, i: int, tid1: int, tid2: int)
+  requires WFSTrace(trace)
+  requires 0 <= i < |trace.edges| - 1
+  requires tid1 in trace.states[i].thread_map
+  requires tid2 in trace.states[i].thread_map
+  requires trace.states[i].thread_map[tid1]
+         > trace.states[i].thread_map[tid2]
+  requires tid1 in trace.states[i].state.threads
+  requires tid2 in trace.states[i].state.threads
+  ensures trace.states[i].state.threads[tid1].lockHeld
+         < trace.states[i].state.threads[tid2].lockHeld;
+  {
+    assert WFSTraceAt(trace, i);
+    assert i > 0;
+    assert WFSTraceAt(trace, i-1);
+    if (trace.edges[i-1].tid == tid1) {
+      if tid1 in trace.states[i-1].state.threads {
+        lock_order(trace, i-1, tid1, tid2);
+
+        assert trace.states[i].state.threads[tid1].lockHeld
+             < trace.states[i].state.threads[tid2].lockHeld;
+      } else {
+        assert trace.states[i].state.threads[tid1].lockHeld
+             < trace.states[i].state.threads[tid2].lockHeld;
+      }
+    } else if (trace.edges[i-1].tid == tid2) {
+      le_largest_so_far(trace, i-1, tid1);
+      assert trace.states[i-1].thread_map[tid1] <= trace.states[i].largest_so_far;
+
+      assert tid2 in trace.states[i-1].thread_map;
+
+      lock_order(trace, i-1, tid1, tid2);
+      assert trace.states[i].state.threads[tid1].lockHeld
+           < trace.states[i].state.threads[tid2].lockHeld;
+    } else {
+      lock_order(trace, i-1, tid1, tid2);
+      assert trace.states[i].state.threads[tid1].lockHeld
+           < trace.states[i].state.threads[tid2].lockHeld;
+    }
+  }
+
+  lemma lt_less_at(trace: STrace, i: int)
+  requires WFSTrace(trace)
+  requires 0 <= i < |trace.edges| - 1
+  requires trace.edges[i].order > trace.edges[i+1].order
+  ensures ConcreteOrdered.lt_less(trace.edges[i].lt, trace.edges[i+1].lt);
+  {
+    var tid1 := trace.edges[i].tid;
+    var tid2 := trace.edges[i+1].tid;
+    assert WFSTraceAt(trace, i);
+    assert WFSTraceAt(trace, i+1);
+
+    order_le_largest_so_far(trace, i);
+    assert trace.edges[i].order <= trace.states[i+1].largest_so_far;
+    assert tid2 in trace.states[i+1].thread_map;
+
+    assert tid1 != tid2; /* by {
+      if tid1 == tid2 {
+        assert tid1 in trace.states[i].thread_map;
+        assert tid1 in trace.states[i+1].thread_map;
+        assert trace.edges[i].order
+            == trace.states[i].thread_map[tid1]
+            == trace.states[i+1].thread_map[tid1]
+            == trace.edges[i+1].order;
+      }
+    }*/
+
+    if (tid2 in trace.states[i].state.threads) {
+      assert trace.states[i].state.threads[tid2]
+          == trace.states[i+1].state.threads[tid2];
+    }
+
+    if (tid1 in trace.states[i].state.threads) {
+      lock_order(trace, i, tid1, tid2);
+      assert trace.states[i].state.threads[tid1].lockHeld
+           < trace.states[i].state.threads[tid2].lockHeld;
+      if (tid1 in trace.states[i+1].state.threads) {
+        assert trace.states[i].state.threads[tid1].lockHeld + 1
+            != trace.states[i].state.threads[tid2].lockHeld;
+      }
+    } else {
+      assert 0
+           < trace.states[i].state.threads[tid2].lockHeld;
+    }
+  }
+
+  lemma do_commute(trace: STrace, i: int) returns (trace': STrace)
+  requires WFSTrace(trace)
+  requires 0 <= i < |trace.edges| - 1
+  requires trace.edges[i].order > trace.edges[i+1].order
+  ensures WFSTrace(trace')
+  {
+    inv_at(trace, i);
+    inv_at(trace, i+1);
+    inv_at(trace, i+2);
+    assert WFSTraceAt(trace, i);
+    assert WFSTraceAt(trace, i+1);
+    lt_less_at(trace, i);
+    var s' := ConcreteOrdered.Commute(
+        trace.states[i].state,
+        trace.states[i+1].state,
+        trace.states[i+2].state,
+        trace.edges[i].tid,
+        trace.edges[i].ui,
+        trace.edges[i].lt,
+        trace.edges[i+1].tid,
+        trace.edges[i+1].ui,
+        trace.edges[i+1].lt);
+
+    var s := trace.states[i];
+    var state';
+    var tid := trace.edges[i+1].tid;
+    if tid in s.state.threads {
+      if tid in s'.threads {
+        state' := SState(s', s.thread_map, s.largest_so_far);
+      } else {
+        state' := SState(
+          s',
+          Concrete.MapRemove1(s.thread_map, tid),
+          s.largest_so_far);
+      }
+    } else {
+      if tid in s'.threads {
+        state' := SState(
+          s',
+          s.thread_map[tid := s.largest_so_far + 1],
+          s.largest_so_far + 1);
+      } else {
+        state' := SState(
+          s',
+          s.thread_map,
+          s.largest_so_far + 1);
+      }
+    }
+    assert ThreadMapUpdate(trace.states[i], state', 
+            trace.edges[i+1].tid, trace.edges[i+1].order);
+    var states' := trace.states[i+1 := state'];
+    var edges' := trace.edges
+        [i := trace.edges[i+1]]
+        [i+1 := trace.edges[i]];
+
+    trace' := STrace(states', edges');
+
+    forall i | 0 <= i < |trace'.edges| ensures WFSTraceAt(trace', i)
+    {
+      assert WFSTraceAt(trace, i);
+    }
+  }
 
   /*lemma Correctness(b:Behavior<Concrete.State>, I:CState->AState)
     requires Reachable(b, Concrete.Init, Concrete.Next)
